Renamed enclaves to counters to be consistent with the paper

examples/preorders/Ariadne.fst
@@ -1,19 +1,19 @@
  module Ariadne
 
-/// CF: We model the Ariadne protocol for state continuity.
-/// https://www.usenix.org/system/files/conference/usenixsecurity16/sec16_paper_strackx.pdf
-///
-/// The protocol ensures that, as the SGX enclaves gets stopped or
-/// its machine crashes, it can be reliably resumed in its last saved
-/// state. The protocol relies on
-/// - a trusted monotonic counter (implemented in hardware, intuitively expensive to increment)
-/// - a trusted fixed key (also implemented in hardware, used for authenticated encryption)
-/// - an untrusted but reliable store on the host, to save encrypted counters & states
+// CF: We model the Ariadne protocol for state continuity.
+// https://www.usenix.org/system/files/conference/usenixsecurity16/sec16_paper_strackx.pdf
+//
+// The protocol ensures that, as the SGX enclave gets stopped or
+// its machine crashes, it can be reliably resumed in its last saved
+// state. The protocol relies on
+// - a trusted monotonic counter (implemented in hardware, intuitively expensive to increment)
+// - a trusted fixed key (also implemented in hardware, used for authenticated encryption)
+// - an untrusted but reliable store on the host, to save encrypted counters & states
 
 open FStar.Preorder
 open FStar.List.Tot
 
-open FStar.All // compared to the accompanying POPL'18 paper, we use F*'s All effect to 
+open FStar.All // Compared to the accompanying POPL'18 paper, we use F*'s All effect to 
                // use the combination of state and exceptions (MSTMSTExn in the paper)
 
 open FStar.Heap
@@ -26,8 +26,8 @@ type state = string // the type of the enclave state; reset on crash.
 
 type record = index * state // the type of records protected by authenticated encryption
 
-/// For the proof, we define a small state machine and its transitions
-/// when sealing and incrementing.
+// For the proof, we define a small state machine and its transitions
+// when sealing and incrementing.
 
 type case = 
   | Ok: saved: state -> case
@@ -41,7 +41,7 @@ type counter =
     c: case -> // ghost state; saves quantifiers
     counter 
 
-/// A monotonic over-approximation of the encrypted records the host may have
+// A monotonic over-approximation of the encrypted records the host may have
 val saved: counter -> record -> Type0
 let saved (Counter n c) s = 
   let m,u = s in 
@@ -58,27 +58,27 @@ let saved (Counter n c) s =
 
 let preorder' :preorder counter = fun (x0:counter) (x1:counter) -> forall s. saved x0 s ==> saved x1 s
 
-type enclave = mref counter preorder' 
+type ctr = mref counter preorder' 
 
-/// An encrypted backup, maintained by the host This is compatible
-/// with our ideal interface for authenticated encryption.
+// An encrypted backup, maintained by the host This is compatible
+// with our ideal interface for authenticated encryption.
 
-let saved_backup (e:enclave) (s:record) = fun h -> h `contains` e /\ saved (sel h e) s
+let saved_backup (c:ctr) (s:record) = fun h -> h `contains` c /\ saved (sel h c) s
 
-type backup (e:enclave) = s:record{witnessed (saved_backup e s)}
+type backup (c:ctr) = s:record{witnessed (saved_backup c s)}
 
-let prefix_of (#e:enclave) (l1:list (backup e)) (l2:list (backup e)) =
+let prefix_of (#c:ctr) (l1:list (backup c)) (l2:list (backup c)) =
   l1 == l2 \/ strict_prefix_of l1 l2
   
-let backups_pre' (e:enclave) :relation (list (backup e)) = fun l1 l2 -> l1 `prefix_of` l2
-let backups_pre (e:enclave) :preorder (list (backup e)) = backups_pre' e
+let backups_pre' (c:ctr) :relation (list (backup c)) = fun l1 l2 -> l1 `prefix_of` l2
+let backups_pre (c:ctr) :preorder (list (backup c)) = backups_pre' c
 
-type backups (e:enclave) = mref (list (backup e)) (backups_pre e) //compared to the general situation described in the
-                                                                 //POPL'18 paper, for simplicity, here we consider only  
-                                                                 //trivial backup keys, i.e., key c = backups c; 
-                                                                 //we omit the auth_encrypt and auth_decrypt functions
+type backups (c:ctr) = mref (list (backup c)) (backups_pre c) // Compared to the general situation described in the
+                                                              // POPL'18 paper, for simplicity, here we consider only  
+                                                              // trivial backup keys, i.e., key c = backups c. Thus, 
+                                                              // we omit the auth_encrypt and auth_decrypt functions
 noeq type protected = 
-  | Protect: e:enclave -> b:backups e -> protected
+  | Protect: c:ctr -> b:backups c -> protected
 
 val create: v: state -> ST protected
   (requires fun h0 -> True)
@@ -90,7 +90,7 @@ let create v =
   let b = alloc [r] in 
   Protect e b 
 
-// privileged code calling back into fallible host code: this may
+// Privileged code calling back into fallible host code: this may
 // fail, in which case we still conservatively assume the host gets
 // the sealed record (although we can't rely on it for recovery)
 
@@ -109,77 +109,77 @@ let step0 c w =
   
 val save: p:protected -> w:state -> All unit 
 (requires fun h0 -> 
-  let Protect e b = p in 
-  pre0 (sel h0 e).c w)
+  let Protect c b = p in 
+  let Counter _ c0 = sel h0 c in 
+  pre0 c0 w)
 (ensures fun h0 r h1 -> 
-  let Protect e b = p in
-  let Counter n c0 = sel h0 e in 
+  let Protect c b = p in
+  let Counter n c0 = sel h0 c in 
   pre0 c0 w /\ (
   let c1 = step0 c0 w in
-  //let log1 = append log0 (n+1,w) in
-  sel h1 e == Counter n c1))
+  sel h1 c == Counter n c1))
 
 let save p w = 
-  let Protect e b = p in
-  let Counter n c0 = read e in
+  let Protect c b = p in
+  let Counter n c0 = read c in
   let c1 = step0 c0 w in
-  write e (Counter n c1); 
+  write c (Counter n c1); 
   let r = (n+1,w) in 
-  witness (saved_backup e r);
+  witness (saved_backup c r);
   let log0 = read b in 
   write b (r::log0)
 
-/// incrementing the counter is privileged code;
-/// it may fail before or after incrementing c
+// Incrementing the counter is privileged code; it may fail before or after incrementing c
 let pre1 c = Writing? c \/ Crash? c
 val step1: c:case {pre1 c} -> case
 let step1 = function
   | Writing w v -> Ok w
   | Crash v0 v1 -> Recover v0 v1
 
-val incr: e:enclave -> w:state -> All unit 
-(requires fun h0 -> pre1 (sel h0 e).c)
+val incr: c:ctr -> w:state -> All unit 
+(requires fun h0 -> 
+  let Counter _ c0 = sel h0 c in
+  pre1 c0)
 (ensures fun h0 r h1 -> 
-  let v0 = sel h0 e in 
+  let v0 = sel h0 c in 
   let Counter n0 c0  = v0 in 
   pre1 c0 /\ (
   let c1 = step1 c0 in 
   let v1 = Counter (n0+1) c1 in 
   match r with 
-  | V _ ->  sel h1 e ==  v1
-  | _ -> sel h1 e == v0 \/ sel h1 e == v1 ))
+  | V _ ->  sel h1 c ==  v1
+  | _ -> sel h1 c == v0 \/ sel h1 c == v1 ))
 
-// sample implementation, with sample failure
-let incr e w = 
-  let x = read e in
+// A sample implementation of incr, with sample failure
+let incr c w = 
+  let x = read c in
   let Counter n0 c0 = x in 
-  if n0 = 3 then failwith "crash" else // else is required!?
-  write e (Counter (n0+1) (step1 c0))
+  if n0 = 3 then failwith "crash" else
+  write c (Counter (n0+1) (step1 c0))
 
-/// storing a checkpoint requires a clean state 
+// storing a checkpoint requires a clean state 
 val store: p:protected -> w:state -> All unit
 (requires fun h0 -> 
-  let Protect e b = p in 
-  Ok? (sel h0 e).c)
+  let Protect c b = p in 
+  let Counter _ c0 = sel h0 c in
+  Ok? c0)
 (ensures fun h0 r h1 -> 
-  let Protect e b = p in
-  let Counter _ c1 = sel h1 e in 
+  let Protect c b = p in
+  let Counter _ c1 = sel h1 c in 
   V? r ==> c1 = Ok w)
   
 let store p w = 
-  let Protect e b = p in 
+  let Protect c b = p in 
   save p w; 
-  incr e w
+  incr c w
 
-/// recovery does not need *any* precondition, and leads to an Ok
-/// state (unless it crashes). We could be more precise, e.g. we never
-/// get None on honest inputs.
-val recover: p:protected -> last_saved:backup (Protect?.e p) -> All (option state)
+// recovery does not need *any* precondition, and leads to an Ok state (unless it crashes)
+val recover: p:protected -> last_saved:backup (Protect?.c p) -> All (option state)
 (requires fun h0 -> True)
 (ensures fun h0 r h1 -> 
-  let Protect e b = p in
-  let Counter _ c0 = sel h0 e in 
-  let Counter _ c1 = sel h1 e in 
+  let Protect c b = p in
+  let Counter _ c0 = sel h0 c in 
+  let Counter _ c1 = sel h1 c in 
   match r with 
   | V None -> h0 == h1
   | V (Some w1) -> (
@@ -187,30 +187,30 @@ val recover: p:protected -> last_saved:backup (Protect?.e p) -> All (option stat
     (match c0 with 
     | Ok w0 -> w1 = w0
     | Writing v0 v0'  | Recover v0 v0' | Crash v0 v0' -> w1 = v0 \/ w1 = v0' ))
-  | _ -> True  // should not be provable?! AR: changed it to True from False, after fixing all_wp in Pervasives
+  | _ -> True
   )
 
 let recover p last_saved = 
-  let Protect e b = p in 
+  let Protect c b = p in 
   let m, w = last_saved in
-  let Counter n c0 = read e in 
+  let Counter n c0 = read c in 
   if m = n  // authenticated decryption
   then ( 
-    recall (saved_backup e last_saved);
+    recall (saved_backup c last_saved);
     save p w;
-    incr e w;
+    incr c w;
     save p w;
-    incr e w;
+    incr c w;
     Some w)
   else None
 
 type trivial 'a = 'a -> All unit (requires fun h0 -> True) (ensures fun h0 _ h1 -> True)
-val example: trivial (trivial enclave)
+val example: trivial (trivial ctr)
 let example attack = 
   let p = create "hello" in
-  let Protect e b = p in
+  let Protect c b = p in
   store p "world";
-  attack e;
+  attack c;
   match read b with 
   | r::_ -> 
     (match recover p r with 
